examples/tls13.v
@@ -660,9 +660,10 @@ iApply Meth.wp_case; case: ke => [psk|g|psk g]; wp_pures.
   do !iSplit => //.
   by iApply "p_cn".
 - iDestruct "p_ke" as "[% p_ke]".
-  wp_bind (mk_dh _); iApply (wp_mk_dh (λ _, True)%I _) => //.
-  { by iApply public_minted. }
-  iIntros (a) "_ #p_a _"; wp_list.
+  wp_bind (mk_dh _); iApply (wp_mk_dh (λ _, True)%I ∅ _) => //.
+  + by iApply public_minted.
+  + by iIntros "!> %"; rewrite elem_of_empty; iIntros ([]).
+  iIntros (a) "_ #p_a _ _"; wp_list.
   wp_bind (mk_nonce _); iApply (wp_mk_nonce (λ _, True)%I (λ _, True)%I) => //.
   iIntros (cn) "_ _ #p_cn _ _ token"; wp_list; wp_term_of_list.
   wp_tag.
@@ -672,9 +673,10 @@ iApply Meth.wp_case; case: ke => [psk|g|psk g]; wp_pures.
   do !iSplit => //.
   by iApply "p_cn".
 - iDestruct "p_ke" as "(? & % & ?)".
-  wp_bind (mk_dh _); iApply (wp_mk_dh (λ _, True)%I _) => //.
-  { by iApply public_minted. }
-  iIntros (a) "_ #p_a _"; wp_list.
+  wp_bind (mk_dh _); iApply (wp_mk_dh (λ _, True)%I ∅ _) => //.
+  + by iApply public_minted.
+  + iIntros "!> %"; rewrite elem_of_empty; iIntros "[]".
+  iIntros (a) "_ #p_a _ _"; wp_list.
   wp_bind (mk_nonce _); iApply (wp_mk_nonce (λ _, True)%I (λ _, True)%I) => //.
   iIntros (cn) "_ _ #p_cn _ _ token"; wp_list; wp_term_of_list.
   wp_tag.
@@ -1145,11 +1147,13 @@ Definition wf ke : iProp :=
     minted psk ∧ public c_nonce ∧ public s_nonce
   | Dh g cn sn gx y =>
     ⌜¬ is_exp g⌝ ∧ public g ∧ public cn ∧ public sn ∧ public gx ∧
+    ⌜∀ x, subterm x gx → y ≠ x ∧ y ≠ TInv x⌝ ∧
     dh_seed (λ _, True)%I y
   | PskDh psk g cn sn gx y =>
     minted psk ∧
     ⌜¬ is_exp g⌝ ∧ public g ∧ public cn ∧ public sn ∧
     public gx ∧
+    ⌜∀ x, subterm x gx → y ≠ x ∧ y ≠ TInv x⌝ ∧
     dh_seed (λ _, True)%I y
   end.
 
@@ -1184,9 +1188,14 @@ case: ke => [psk' cn|g' cn gx|psk' g' cn gx] /= in e_check *; wp_pures.
   do !iSplit => //.
   by iApply "pred_a".
 - subst g'.
-  wp_bind (mk_dh _); iApply (wp_mk_dh (λ _, True)%I _) => //.
-  { by iApply public_minted. }
-  iIntros (a) "_ #pred_a _"; wp_list.
+  wp_bind (mk_dh _); iApply (wp_mk_dh (λ _, True)%I {[gx]} _) => //.
+  + by iApply public_minted.
+  + iIntros "!> %t"; iIntros (->%elem_of_singleton); rewrite !public_minted.
+    rewrite minted_tag minted_of_list /=.
+    by iDestruct "p_ke" as "(_ & _ & ? & _)".
+  iIntros (a) "_ #pred_a _ %fresh_a"; wp_list.
+  have {}fresh_a: ∀ t, subterm t gx → a ≠ t ∧ a ≠ TInv t.
+    by move=> t; apply: fresh_a; set_solver.
   wp_bind (mk_nonce _); iApply (wp_mk_nonce (λ _, True)%I (λ _, True)%I) => //.
   iIntros (sn) "_ _ #p_sn _ _ token"; wp_list; wp_term_of_list.
   wp_tag; iModIntro.
@@ -1196,9 +1205,14 @@ case: ke => [psk' cn|g' cn gx|psk' g' cn gx] /= in e_check *; wp_pures.
   do !iSplit => //.
   by iApply "p_sn".
 - case: e_check=> -> ->.
-  wp_bind (mk_dh _); iApply (wp_mk_dh (λ _, True)%I _) => //.
-  { by iApply public_minted. }
-  iIntros (a) "_ #pred_a _"; wp_list.
+  wp_bind (mk_dh _); iApply (wp_mk_dh (λ _, True)%I {[gx]} _) => //.
+  + by iApply public_minted.
+  + iIntros "!> %t"; iIntros (->%elem_of_singleton); rewrite !public_minted.
+    rewrite minted_tag minted_of_list /=.
+    by iDestruct "p_ke" as "(_ & _ & _ & ? & _)".
+  iIntros (a) "_ #pred_a _ %fresh_a"; wp_list.
+  have {}fresh_a: ∀ t, subterm t gx → a ≠ t ∧ a ≠ TInv t.
+    by move=> t; apply: fresh_a; set_solver.
   wp_bind (mk_nonce _); iApply (wp_mk_nonce (λ _, True)%I (λ _, True)%I) => //.
   iIntros (sn) "_ _ #p_sn _ _ token"; wp_list; wp_term_of_list.
   wp_tag; iModIntro.
@@ -1265,11 +1279,11 @@ case: ke=>> /=.
   rewrite public_THash; iRight.
   rewrite minted_tag; iSplit => //.
   by iExists _, _, _; eauto.
-- iIntros "#(% & p_g & p_cn & p_sn & p_gx & seed_y)".
+- iIntros "#(% & p_g & p_cn & p_sn & p_gx & _ & seed_y)".
   rewrite public_tag public_of_list /=.
   do !iSplit => //.
   by iApply dh_public_TExp; eauto.
-- iIntros "#(p_psk & % & p_g & p_cn & p_sn & p_gx & seed_y)".
+- iIntros "#(p_psk & % & p_g & p_cn & p_sn & p_gx & _ & seed_y)".
   rewrite public_tag public_of_list /=.
   do !iSplit => //.
   + rewrite public_THash; iRight.
@@ -1283,11 +1297,11 @@ Proof.
 case: ke=>> /=.
 - iIntros "#(?&?&?)".
   rewrite minted_senc minted_of_list /=; do !iSplit; eauto.
-- iIntros "#(%&?&?&?&?&seed)".
+- iIntros "#(%&?&?&?&?&_&seed)".
   rewrite minted_senc; iApply all_minted_TExp; eauto.
   iDestruct "seed" as "(?&_)".
   by iSplit => //; iApply public_minted.
-- iIntros "#(?&%&?&?&?&?&seed)".
+- iIntros "#(?&%&?&?&?&?&_&seed)".
   rewrite minted_senc minted_of_list /=; do !iSplit => //.
   iApply all_minted_TExp; eauto.
   iDestruct "seed" as "(?&_)".
@@ -1329,24 +1343,28 @@ Proof.
 iIntros (e) "#wf1 #wf2 #p_k". rewrite public_senc_key.
 case: c_kex e => [psk cn sn|g cn sn x gy|psk g cn sn x gy] /=.
 - case: s_kex => //= _ _ _ [] /Spec.tag_inj [_ <-] <- <-.
-  rewrite public_of_list /=. iDestruct "p_k" as "(?&?&?&_)". by eauto.
+  by rewrite public_of_list /=; iDestruct "p_k" as "(?&?&?&_)"; eauto.
 - case: s_kex => //= _ ? ? gx y [] <- _ _ <- e2.
-  iDestruct "wf1" as "#(% & _ & _ & dh_x)".
-  iDestruct "wf2" as "#(_ & _ & _ & _ & p_gx & dh_y)".
+  iDestruct "wf1" as "#(%gXN & _ & _ & dh_x)".
+  move/negb_True: (gXN) => ?.
+  iDestruct "wf2" as "#(_ & _ & _ & _ & p_gx & %fresh_y & dh_y)".
+  have [??]: y ≠ x ∧ y ≠ TInv x.
+    apply: fresh_y; apply: STExp2; eauto; first exact: invs_canceled1.
+    set_solver.
   rewrite /session_key_of TExp_TExpN.
-  iMod (dh_seed_elim2 with "dh_y dh_x p_k") as "(%e & _ & _)" => //.
-  + admit.
-  + admit.
+  by iMod (dh_seed_elim2 with "dh_y dh_x p_k") as "[]".
 - case: s_kex => //= _ ? ? ? gx y [] /Spec.tag_inj [_ <-].
   move=> <- _ _ <- e2.
-  iDestruct "wf1" as "#(_ & % & _ & _ & dh_x)".
-  iDestruct "wf2" as "#(_ & _ & _ & _ & _ & p_gx & dh_y)".
+  iDestruct "wf1" as "#(_ & %gXN & _ & _ & dh_x)".
+  move/negb_True: (gXN) => ?.
+  iDestruct "wf2" as "#(_ & _ & _ & _ & _ & p_gx & %fresh_y & dh_y)".
+  have [??]: y ≠ x ∧ y ≠ TInv x.
+    apply: fresh_y; apply: STExp2; eauto; first exact: invs_canceled1.
+    set_solver.
   rewrite TExp_TExpN.
   rewrite public_of_list /=. iDestruct "p_k" as "(_ & p_k & _)".
-  iMod (dh_seed_elim2 with "dh_y dh_x p_k") as "(%e & _ & _)" => //.
-  + admit.
-  + admit.
-Admitted.
+  by iMod (dh_seed_elim2 with "dh_y dh_x p_k") as "[]".
+Qed.
 
 End Proofs.
 
